ocaml, coq: Complete implementation of the frontend

ocaml/SGALib.ml
@@ -31,7 +31,7 @@ module Util = struct
       | SGA.UnboundVariable var ->
          (`NameError, Printf.sprintf "Unbound variable `%s'" var)
       | SGA.TypeMismatch (_tsig, actual, _expr, expected) ->
-         (`TypeError, Printf.sprintf "Inferred type %s does not match expected type %s"
+         (`TypeError, Printf.sprintf "This term has type `%s', but `%s' was expected"
                         (type_to_string actual) (type_to_string expected))
     in Error { epos = epos; ekind = ekind; emsg = emsg }
 
@@ -42,10 +42,23 @@ module Util = struct
   let bits_const_to_int bs =
     List.fold_right (fun b bs -> (if b then 1 else 0) + 2 * bs) bs.bs_bits 0
 
-  let dedup_input_of_tc_unit { tc_registers; _ } circuits =
+  let ffi_signature_of_interop_fn ffi_name (fsig: SGA.externalSignature) =
+    { ffi_name;
+      ffi_arg1size = fsig.arg1Type;
+      ffi_arg2size = fsig.arg2Type;
+      ffi_retsize = fsig.retType }
+
+  let dedup_input_of_tc_unit { tc_registers } circuits =
     { di_regs = tc_registers;
       di_reg_sigs = (fun r -> r);
-      di_fn_sigs = (fun fn -> fn);
+      di_fn_sigs = (fun fn ->
+        let ffi_name, fsig = match fn with
+          | SGA.PrimFn fn ->
+             PrimFn fn,
+             SGA.prim_Sigma fn
+          | SGA.CustomFn _ ->
+             failwith "No custom functions" in
+        ffi_signature_of_interop_fn ffi_name fsig);
       di_circuits = circuits }
 
   let dedup_input_of_verilogPackage (pkg: SGA.verilogPackage) =
@@ -64,45 +77,121 @@ module Util = struct
       | SGA.CustomFn fn ->
          CustomFn (string_of_coq_string (pkg.vp_custom_fn_names fn)),
          pkg.vp_custom_fn_types fn in
-      { ffi_name;
-        ffi_arg1size = fsig.arg1Type;
-        ffi_arg2size = fsig.arg2Type;
-        ffi_retsize = fsig.retType } in
+      ffi_signature_of_interop_fn ffi_name fsig in
     let di_circuits r =
       SGA.getenv pkg.vp_reg_Env pkg.vp_circuit r in
     { di_regs; di_reg_sigs; di_fn_sigs; di_circuits }
 end
 
 module Compilation = struct
-  let translate_expr_ast raw_ast =
-    Obj.magic ()
+  module DebugPrinter = struct
+    open SGA
+    open Printf
 
-  let translate_rule_ast raw_ast =
-    Obj.magic ()
+    let pp_port = function
+      | P0 -> "P0"
+      | P1 -> "P1"
 
-  let translate_scheduler_ast raw_ast =
-    Obj.magic ()
+    let rec pp_expr = function
+      | UVar v -> sprintf "var %s" v
+      | UConst (n, bs) ->
+         sprintf "%d'%s" n
+           (String.concat "" (List.rev_map (fun x -> if x then "1" else "0") (SGA.vect_to_list n bs)))
+      | URead (p, r) -> sprintf "%s.read#%s" r.reg_name (pp_port p)
+      | UCall (_, e1, e2) -> (sprintf "UCall (__, %s, %s)" (pp_expr e1) (pp_expr e2))
+      | UEPos (_, x) -> pp_expr x
+
+    let rec pp_rule = function
+      | USkip -> "Skip"
+      | UFail -> "Fail"
+      | USeq (r1, r2) -> sprintf "Seq (%s) (%s)" (pp_rule r1) (pp_rule r2)
+      | UBind (v, e, r) -> sprintf "Bind (%s <- %s) (%s)" v (pp_expr e) (pp_rule r)
+      | UIf (c, r1, r2) -> sprintf "If %s Then %s Else %s EndIf" (pp_expr c) (pp_rule r1) (pp_rule r2)
+      | UWrite (p, r, v) -> sprintf "%s.write#%s(%s)" r.reg_name (pp_port p) (pp_expr v)
+      | URPos (_, x) -> pp_rule x
+
+    let rec pp_scheduler = function
+      | UDone -> "Done"
+      | UTry (r, s1, s2) -> sprintf "Try (%s) (%s) (%s)" (pp_rule r) (pp_scheduler s1) (pp_scheduler s2)
+      | USPos (_, x) -> pp_scheduler x
+  end
+
+  let translate_port = function
+    | 0 -> SGA.P0
+    | 1 -> SGA.P1
+    | _ -> assert false
+
+  let rec translate_expr { lpos; lcnt } =
+    SGA.UEPos
+      (lpos,
+       match lcnt with
+       | Var v -> SGA.UVar v
+       | Num _ -> assert false
+       | Const bs -> SGA.UConst (List.length bs, SGA.vect_of_list bs)
+       | Read (port, reg) -> SGA.URead (translate_port port, reg.lcnt)
+       | Call (fn, a1 :: a2 :: []) -> SGA.UCall (fn.lcnt, translate_expr a1, translate_expr a2)
+       | Call (_, _) -> assert false)
+
+  let rec translate_rule { lpos; lcnt } =
+    SGA.URPos
+      (lpos,
+       match lcnt with
+       | Skip -> SGA.USkip
+       | Fail -> SGA.UFail
+       | Progn rs -> translate_seq rs
+       | Let (bs, body) -> translate_bindings bs body
+       | If (e, r, rs) -> SGA.UIf (translate_expr e, translate_rule r, translate_seq rs)
+       | When (e, rs) -> SGA.UIf (translate_expr e, translate_seq rs, SGA.UFail)
+       | Write (port, reg, v) ->
+          SGA.UWrite (translate_port port, reg.lcnt, translate_expr v))
+  and translate_bindings bs body =
+    match bs with
+    | [] -> translate_seq body
+    | (v, e) :: bs -> SGA.UBind (v.lcnt, translate_expr e, translate_bindings bs body)
+  and translate_seq rs =
+    match rs with
+    | [] -> SGA.USkip
+    | [r] -> translate_rule r
+    | r :: rs -> SGA.USeq (translate_rule r, translate_seq rs)
+
+  let rec translate_scheduler { lpos; lcnt } =
+    SGA.USPos
+      (lpos,
+       match lcnt with
+       | ADone -> SGA.UDone
+       | ASequence [] -> SGA.UDone
+       | ASequence (r :: rs) ->
+          let s' = translate_scheduler { lpos; lcnt = ASequence rs } in
+          SGA.UTry (translate_rule r, s', s')
+       | ATry (r, s1, s2) ->
+          SGA.UTry (translate_rule r,
+                    translate_scheduler s1,
+                    translate_scheduler s2))
 
   let r = fun rs ->
     rs.reg_size
 
   let sigma = fun fn ->
-    { SGA.arg1Type = fn.ffi_arg1size;
-      SGA.arg2Type = fn.ffi_arg2size;
-      SGA.retType = fn.ffi_retsize }
+    SGA.interop_Sigma (fun _ -> failwith "No custom functions") fn
 
-  let rEnv_of_tc_unit { tc_registers; _ } =
+  let uSigma = fun fn ->
+    SGA.interop_uSigma (fun _ -> failwith "No custom functions") fn
+
+  let rEnv_of_register_list tc_registers =
     let eqdec r1 r2 = Util.string_eq_dec r1.reg_name r2.reg_name in
     SGA.contextEnv { SGA.finite_elems = tc_registers; (* TODO memoize call to mem *)
                      SGA.finite_index = fun rn -> match SGA.mem eqdec rn tc_registers with
                                                   | Inl m -> m
                                                   | Inr _ -> failwith "Unexpected register name" }
 
-  let compile tc_unit raw_ast : (reg_signature -> (reg_signature, 'prim ffi_signature) SGA.circuit) =
-    let ast = translate_scheduler_ast raw_ast in
-    let rEnv = rEnv_of_tc_unit tc_unit in
-    let r0: _ SGA.env_t = rEnv.create __ (fun r -> Obj.magic (CReadRegister r)) in
-    match SGA.type_scheduler Util.string_eq_dec r sigma Lexing.dummy_pos ast with
+  let compile
+        (tcu: tc_unit)
+        (ast: string SGA.interop_ufn_t ast locd)
+      : (reg_signature -> (reg_signature, string SGA.interop_fn_t) SGA.circuit) =
+    let ast = translate_scheduler ast in
+    let rEnv = rEnv_of_register_list tcu.tc_registers in
+    let r0: _ SGA.env_t = SGA.create rEnv (fun r -> SGA.CReadRegister r) in
+    match SGA.type_scheduler Util.string_eq_dec r sigma uSigma Lexing.dummy_pos ast with
     | WellTyped s ->
        let env = SGA.compile_scheduler r sigma rEnv r0 s in
        (fun r -> SGA.getenv rEnv env r)
@@ -111,14 +200,14 @@ module Compilation = struct
 end
 
 module Graphs = struct
-  module CircuitHash =
-    struct
-      type t = Obj.t
-      let equal o1 o2 = o1 == o2
-      let hash o = Hashtbl.hash o
-    end
+  (* module CircuitHash =
+   *   struct
+   *     type t = Obj.t
+   *     let equal o1 o2 = o1 == o2
+   *     let hash o = Hashtbl.hash o
+   *   end *)
 
-  module CircuitHashtbl = Hashtbl.Make(CircuitHash)
+  module CircuitHashtbl = Hashtbl
 
   type 'prim circuit_graph = {
       graph_roots: circuit_root list;
@@ -130,8 +219,9 @@ module Graphs = struct
     let ptr_to_object = PtrHashtbl.create 50 in
     let nextptr = ref 0 in
     let rec aux (c: _ SGA.circuit) =
-      match CircuitHashtbl.find_opt circuit_to_ptr (Obj.magic c) with
-      | Some ptr -> ptr
+      match CircuitHashtbl.find_opt circuit_to_ptr c with
+      | Some ptr ->
+         ptr
       | None ->
          let ptr = !nextptr in
          incr nextptr;
@@ -154,7 +244,7 @@ module Graphs = struct
            | SGA.CAnnot (sz, annot, c) ->
               CAnnot (sz, Util.string_of_coq_string annot, aux c)
          in
-         CircuitHashtbl.add circuit_to_ptr (Obj.magic c) ptr;
+         CircuitHashtbl.add circuit_to_ptr c ptr;
          PtrHashtbl.add ptr_to_object ptr deduplicated;
          ptr in
     (* CircuitHashtbl.fold (fun k v acc -> (k, v) :: acc)  object_to_ptr [], *)
