ocaml/cli.ml
@@ -1,19 +1,361 @@
 open Common
 
-let ast_of_tokens tokens =
-  Obj.magic ()
+type smod = {
+    m_name: string locd;
+    m_args: string locd list;
+    m_registers: (string locd * bool list locd) list;
+    m_rules: (string locd * (string, string) rule locd) list;
+    m_scheduler: string locd * scheduler locd
+  }
 
-let tokens_of_stream stream =
-  Obj.magic ()
+let sprintf = Printf.sprintf
 
-let stream_of_fname fname =
-  Obj.magic ()
+let parse_error (epos: Lexing.position) emsg =
+  raise (Error { epos; ekind = `ParseError; emsg })
+
+let name_error (epos: Lexing.position) kind name =
+  raise (Error { epos; ekind = `NameError;
+                 emsg = sprintf "Unbound %s: `%s'" kind name })
+
+let type_error (epos: Lexing.position) emsg =
+  raise (Error { epos; ekind = `TypeError; emsg })
+
+let untyped_number_error (epos: Lexing.position) n =
+  type_error epos (sprintf "Missing size annotation on number `%d'" n)
+
+let expect_cons loc msg = function
+  | [] ->
+     parse_error loc (Printf.sprintf "Missing %s" msg)
+  | hd :: tl -> hd, tl
+
+let rec list_const n x =
+  if n = 0 then [] else x :: list_const (n - 1) x
 
 let parse fname =
-  fname
-  |> stream_of_fname
-  |> tokens_of_stream
-  |> ast_of_tokens
+  Printf.printf "Parsing %s\n%!" fname;
+  let open Parsexp in
+  let open Positions in
+  let open Parsexp.Cst in
+  let drop_comments =
+    Base.List.filter_map ~f:(function Sexp s -> Some s | _ -> None) in
+  let epos_of_pos (pos: Positions.pos) =
+    Lexing.{ pos_fname = fname; pos_bol = pos.offset - pos.col;
+             pos_lnum = pos.line; pos_cnum = pos.offset } in
+  let epos_of_range loc =
+    epos_of_pos loc.start_pos in
+  let parse_error (loc: range) msg =
+    parse_error (epos_of_range loc) msg in
+  let expect_cons loc msg =
+    expect_cons (epos_of_range loc) msg in
+  let expect_single loc kind where = function
+    | [] ->
+       parse_error loc
+         (sprintf "No %s found in %s" kind where)
+    | _ :: _ :: _ ->
+       parse_error loc
+         (sprintf "More than one %s found in %s" kind where)
+    | [x] -> x in
+  let locd_make (rng: range) x =
+    { lpos = epos_of_pos rng.start_pos; lcnt = x } in
+  let locd_of_pair (pos, x) =
+    locd_make pos x in
+  let read_sexps fname =
+    match Parsexp.Many_cst.parse_string (Stdio.In_channel.read_all fname) with
+    | Ok sexps ->
+       drop_comments sexps
+    | Error err ->
+       let pos = Parsexp.Parse_error.position err in
+       let msg = Parsexp.Parse_error.message err in
+       parse_error { start_pos = pos; end_pos = pos } msg in
+  let num_fmt =
+    "(number format: size'number)" in
+  let expect_atom msg = function
+    | Cst.List { loc; _ } ->
+       parse_error loc
+         (sprintf "Expecting %s, but got a list" msg)
+    | Cst.Atom { loc; atom; _ } ->
+       (loc, atom) in
+  let expect_list msg = function
+    | Cst.Atom { loc; atom; _ } ->
+       parse_error loc
+         (sprintf "Expecting %s, but got `%s'" msg atom)
+    | Cst.List { loc; elements } ->
+       (loc, drop_comments elements) in
+  let expect_nil = function
+    | [] -> ()
+    | Cst.List { loc; _ } :: _ -> parse_error loc "Unexpected list"
+    | Cst.Atom { loc; _ } :: _ -> parse_error loc "Unexpected atom" in
+  let expect_constant csts c =
+    let quote x = "`" ^ x ^ "'" in
+    let optstrs = List.map (fun x -> quote (fst x)) csts in
+    let msg = sprintf "one of %s" (String.concat ", " optstrs) in
+    let loc, s = expect_atom msg c in
+    match List.assoc_opt s csts with
+    | None -> parse_error loc (sprintf "Expecting %s, got `%s'" msg s)
+    | Some x -> loc, x in
+  let bits_const_re =
+    Str.regexp "^\\([0-9]+\\)'\\(0b[01]*\\|0x[0-9A-F]*\\|[0-9]+\\)$" in
+  let ident_re =
+    Str.regexp "^[a-z][a-zA-Z0-9_]*$" in
+  let try_variable var =
+    if Str.string_match ident_re var 0 then Some var else None in
+  let try_number loc a =
+    if Str.string_match bits_const_re a 0 then
+      let sizestr = Str.matched_group 1 a in
+      let size = try int_of_string sizestr
+                 with Failure _ ->
+                   parse_error loc (sprintf "Unparsable size annotation: `%s'" sizestr) in
+      let numstr = Str.matched_group 2 a in
+      let num = Z.of_string numstr in
+      let bits = if size = 0 && num = Z.zero then []
+                 else List.of_seq (String.to_seq (Z.format "%b" num)) in
+      let nbits = List.length bits in
+      if nbits > size then
+        parse_error loc (sprintf "Number `%s' does not fit in %d bit(s)" numstr size)
+      else
+        let padding = list_const (size - nbits) false in
+        let char2bool = function '0' -> false | '1' -> true | _ -> assert false in
+        let bools = List.append (List.rev_map char2bool bits) padding in
+        Some (Const bools)
+    else match int_of_string_opt a with
+         | Some n -> Some (Num n)
+         | None -> None in
+  let expect_number_or_var loc a =
+    match try_number loc a with
+    | Some c -> c
+    | None ->
+       match try_variable a with
+       | Some var -> Var var
+       | None ->
+          let msg = sprintf "Cannot parse `%s' as a number or identifier %s" a num_fmt in
+          parse_error loc msg in
+  let expect_funapp loc kind elements =
+    let hd, args = expect_cons loc kind elements in
+    let loc_hd, hd = expect_atom (sprintf "a %s name" kind) hd in
+    loc_hd, hd, args in
+  let rec expect_expr = function
+    | Cst.Atom { loc; atom; _ } ->
+       locd_make loc (expect_number_or_var loc atom)
+    | Cst.List { loc; elements } ->
+       let loc_hd, hd, args = expect_funapp loc "constructor or function" (drop_comments elements) in
+       locd_make loc
+         (match hd with
+          | "read#0" | "read#1" ->
+             let reg, body = expect_cons loc "register name" args in
+             let port = int_of_string (String.sub hd (String.length hd - 1) 1) in
+             let () = expect_nil body in
+             Read (port, locd_of_pair (expect_atom "a register name" reg))
+          | _ ->
+             let args = List.map expect_expr args in
+             Call (locd_make loc_hd hd, args)) in
+  let expect_let_binding b =
+    let loc, b = expect_list "a let binding" b in
+    let var, values = expect_cons loc "identifier" b in
+    let loc_v, var = expect_atom "an identifier" var in
+    match try_variable var with
+    | None -> parse_error loc_v (sprintf "Cannot parse `%s' as an identifier" var)
+    | Some var ->
+       let value = expect_single loc "value" "let binding" values in
+       let value = expect_expr value in
+       (locd_make loc_v var, value) in
+  let expect_let_bindings bs =
+    let _, bs = expect_list "let bindings" bs in
+    List.map expect_let_binding bs in
+  let expect_register init_val =
+    (* let loc, taus = expect_list "a type declaration" taus in
+     * let bit, sizes = expect_cons loc "a type declaration" taus in
+     * let _ = expect_constant [("bit", ())] bit in
+     * let size = expect_single loc "size" "type declaration" sizes in
+     * let sloc, size = expect_atom "size" size in
+     * try locd_make sloc (int_of_string size)
+     * with Failure _ ->
+     *   parse_error loc (sprintf "Unparsable size %s" size) in *)
+    let loc, init_val = expect_atom "an initial value" init_val in
+    match try_number loc init_val with
+    | Some (Const c) -> locd_make loc c
+    | Some (Num n) -> untyped_number_error (epos_of_range loc) n
+    | _ -> parse_error loc (sprintf "Expecting a number, got `%s' %s" init_val num_fmt) in
+  let rec expect_rule = function
+    | (Cst.Atom _) as a ->
+       locd_of_pair (expect_constant [("skip", Skip); ("fail", Fail)] a)
+    | Cst.List { loc; elements } ->
+       let loc_hd, hd, args = expect_funapp loc "constructor" (drop_comments elements) in
+       locd_make loc
+         (match hd with
+          | "progn" ->
+             Progn (List.map expect_rule args)
+          | "let" ->
+             let bindings, body = expect_cons loc "let bindings" args in
+             Let (expect_let_bindings bindings, List.map expect_rule body)
+          | "if" ->
+             let cond, body = expect_cons loc "if condition" args in
+             let tbranch, fbranches = expect_cons loc "if branch" body in
+             If (expect_expr cond, expect_rule tbranch,
+                 List.map expect_rule fbranches)
+          | "when" ->
+             let cond, body = expect_cons loc "when condition" args in
+             When (expect_expr cond, List.map expect_rule body)
+          | "write#0" | "write#1" ->
+             let reg, body = expect_cons loc "register name" args in
+             let port = int_of_string (String.sub hd (String.length hd - 1) 1) in
+             Write (port, locd_of_pair (expect_atom "a register name" reg),
+                    expect_expr (expect_single loc "value" "write expression" body))
+          | _ ->
+             parse_error loc_hd (sprintf "Unexpected in rule: `%s'" hd)) in
+  let rec expect_scheduler : Cst.t -> scheduler locd = function
+    | (Cst.Atom _) as a ->
+       locd_of_pair (expect_constant [("done", Done)] a)
+    | Cst.List { loc; elements } ->
+       let loc_hd, hd, args = expect_funapp loc "constructor" (drop_comments elements) in
+       locd_make loc
+         (match hd with
+          | "sequence" ->
+             Sequence (List.map (fun a -> locd_of_pair (expect_atom "a rule name" a)) args)
+          | "try" ->
+             let rname, args = expect_cons loc "rule name" args in
+             let s1, args = expect_cons loc "subscheduler 1" args in
+             let s2, args = expect_cons loc "subscheduler 2" args in
+             let _ = expect_nil args in
+             Try (locd_of_pair (expect_atom "a rule name" rname),
+                  expect_scheduler s1,
+                  expect_scheduler s2)
+          | _ ->
+             parse_error loc_hd (sprintf "Unexpected in scheduler: `%s'" hd)) in
+  let rec expect_decl d =
+    let d_loc, d = expect_list "a rule or scheduler declaration" d in
+    let kind, name_body = expect_cons d_loc "rule or scheduler declaration" d in
+    let csts = [("rule", `Rule); ("scheduler", `Scheduler);
+                ("register", `Register); ("module", `Module)] in
+    let _, kind = expect_constant csts kind in
+    let name, body = expect_cons d_loc "name" name_body in
+    let name = locd_of_pair (expect_atom "a name" name) in
+    Printf.printf "Processing decl %s\n%!" name.lcnt;
+    (d_loc,
+     match kind with
+     | `Register ->
+        `Register (name, expect_register (expect_single d_loc "type" "register declaration" body))
+     | `Module ->
+        `Module (expect_module name d_loc body)
+     | `Rule ->
+        `Rule (name, expect_rule (expect_single d_loc "body" "rule declaration" body))
+     | `Scheduler ->
+        `Scheduler (name, expect_scheduler (expect_single d_loc "body" "scheduler declaration" body)))
+  and expect_module m_name m_loc args_body =
+    let args, body = expect_cons m_loc "module arguments" args_body in
+    let _, args = expect_list "module arguments" args in
+    let m_args = List.map (fun a -> locd_of_pair (expect_atom "an argument name" a)) args in
+    let m_registers, m_rules,  schedulers =
+      List.fold_left (fun (registers, rules, schedulers) decl ->
+          match expect_decl decl with
+          | _, `Register r -> (r :: registers, rules, schedulers)
+          | _, `Rule r -> (registers, r :: rules, schedulers)
+          | _, `Scheduler s -> (registers, rules, s :: schedulers)
+          | loc, `Module _ -> parse_error loc "Unexpected nested module declaration")
+        ([], [], []) body in
+    let m_scheduler = expect_single m_loc "scheduler"
+                        (sprintf "module `%s'" m_name.lcnt) schedulers in
+    { m_name; m_args; m_registers; m_rules; m_scheduler } in
+  let compute_tc_unit { m_registers; m_rules; m_scheduler; _ } =
+    let tc_unit =
+      { tc_registers = List.map (fun (nm, init) ->
+                           let bs_size = List.length init.lcnt in
+                           { reg_name = nm.lcnt;
+                             reg_size = bs_size;
+                             reg_init_val = { bs_size; bs_bits = init.lcnt } })
+                         m_registers } in
+    (* FIXME: handle functions in generic way *)
+    (tc_unit, m_rules, m_scheduler) in
+  let sexps =
+    read_sexps fname in
+  List.map (fun sexp ->
+      match expect_decl sexp with
+      | _, `Module m -> compute_tc_unit m
+      | loc, kind ->
+         parse_error loc (sprintf "Unexpected %s at top level"
+                            (match kind with
+                             | `Register _ -> "register"
+                             | `Module _ -> assert false
+                             | `Rule _ -> "rule"
+                             | `Scheduler _ -> "scheduler")))
+    sexps
+
+let resolve tcu rules scheduler =
+  let find_register { lpos; lcnt = name } =
+    match List.find_opt (fun rsig -> rsig.reg_name = name) tcu.tc_registers with
+    | Some rsig -> { lpos; lcnt = rsig }
+    | None -> name_error lpos "register" name in
+  let w0 = { lpos = Lexing.dummy_pos; lcnt = Const [] } in
+  let find_function { lpos; lcnt = name } args =
+    (* FIXME generalize to custom function definitions *)
+    let (fn, nargs, args): SGALib.SGA.prim_ufn_t * int * _ =
+      match name with
+      | "sel" -> USel, 2, args
+      | "and" -> UAnd, 2, args
+      | "or" -> UOr, 2, args
+      | "not" -> UNot, 1, args
+      | "lsl" -> ULsl, 2, args
+      | "lsr" -> ULsr, 2, args
+      | "eq" -> UEq, 2, args
+      | "concat" -> UConcat, 2, args
+      | "uintplus" | "+" -> UUIntPlus, 2, args
+      | "part" | "zextl" | "zextr" ->
+         (match expect_cons lpos "argument" args with
+          | { lcnt = Num n; _}, args ->
+             (match name with
+              | "part" -> UPart n, 2, args
+              | "zextl" -> UZExtR n, 2, args
+              | "zextr" -> UZExtL n, 2, args
+              | _ -> assert false)
+          | { lpos; _ }, _ -> parse_error lpos "Expecting a type-level constant")
+      | _ -> name_error lpos "function" name in
+    assert (nargs <= 2);
+    if List.length args <> nargs then
+      type_error lpos (sprintf "Function `%s' takes %d arguments" name nargs)
+    else
+      let padding = list_const (2 - nargs) w0 in
+      { lpos; lcnt = SGALib.SGA.UPrimFn fn }, List.append args padding in
+  let rec resolve_expr ({ lpos; lcnt }: (string, string) expr locd) =
+    { lpos;
+      lcnt = match lcnt with
+             | Var v -> Var v
+             | Num n -> untyped_number_error lpos n
+             | Const bs -> Const bs
+             | Read (port, r) ->
+                Read (port, find_register r)
+             | Call (fn, args) ->
+                let fn, args = find_function fn args in
+                Call (fn, List.map resolve_expr args) } in
+  let rec resolve_rule ({ lpos; lcnt }: (string, string) rule locd) =
+    { lpos;
+      lcnt = match lcnt with
+             | Skip -> Skip
+             | Fail -> Fail
+             | Progn rs -> Progn (List.map resolve_rule rs)
+             | Let (bs, body) ->
+                Let (List.map (fun (var, expr) -> (var, resolve_expr expr)) bs,
+                     List.map resolve_rule body)
+             | If (c, l, rs) ->
+                If (resolve_expr c,
+                    resolve_rule l,
+                    List.map resolve_rule rs)
+             | When (c, rs) ->
+                When (resolve_expr c, List.map resolve_rule rs)
+             | Write (port, r, v) ->
+                Write (port, find_register r, resolve_expr v) } in
+  let rules = List.map (fun (nm, r) -> (nm, resolve_rule r)) rules in
+  let find_rule { lpos; lcnt = name } =
+    match List.find_opt (fun (nm, _) -> nm.lcnt = name) rules with
+    | Some (_, { lcnt; _ }) -> { lpos; lcnt }
+    | None -> name_error lpos "rule" name in
+  let rec resolve_scheduler ({ lpos; lcnt }: scheduler locd) =
+    { lpos; (* FIXME add support for calling other schedulers by name *)
+      lcnt = match lcnt with
+             | Done -> ADone
+             | Sequence rs ->
+                ASequence (List.map find_rule rs)
+             | Try (r, s1, s2) ->
+                ATry (find_rule r, resolve_scheduler s1, resolve_scheduler s2) } in
+  resolve_scheduler scheduler
 
 type cli_opts = {
     cli_in_fname: string;
@@ -21,40 +363,24 @@ type cli_opts = {
     cli_backend: [`Dot | `Verilog]
   }
 
-let cli (k: cli_opts -> unit) =
-  let open Core in
-  let open Command.Spec in
-  let open Command.Param in
-  let backend_of_fname fname =
-    match Core.Filename.split_extension fname with
-    | _, Some ".v" -> `Verilog
-    | _, Some ".dot" -> `Dot
-    | _, _ -> failwith "Unsupported extension" in
-  Command.basic
-    ~summary:"Compile simultaneous guarded actions to a circuit"
-    Command.Let_syntax.(
-    let%map_open
-        cli_in_fname = anon ("input" %: string)
-    and cli_out_fname = anon ("output" %: string)
-    in fun () ->
-       k { cli_in_fname; cli_out_fname;
-           cli_backend = backend_of_fname cli_out_fname })
-
 let run { cli_in_fname; cli_out_fname; cli_backend } : unit =
   try
-    let tc_unit, ast =
-      parse cli_in_fname in
-    let circuits =
-      SGALib.Compilation.compile tc_unit ast in
-    let graph =
-      SGALib.Graphs.dedup_circuit (SGALib.Util.dedup_input_of_tc_unit tc_unit circuits) in
-    Stdio.Out_channel.with_file cli_out_fname ~f:(fun out ->
-        match cli_backend with
-        | `Dot -> Backends.Dot.main out graph
-        | `Verilog -> Backends.Verilog.main out graph)
+    (match parse cli_in_fname with
+     | (tc_unit, rules, scheduler) :: _ ->
+        let ast =
+          resolve tc_unit rules (snd scheduler) in
+        let circuits =
+          SGALib.Compilation.compile tc_unit ast in
+        let graph =
+          SGALib.Graphs.dedup_circuit (SGALib.Util.dedup_input_of_tc_unit tc_unit circuits) in
+        Stdio.Out_channel.with_file cli_out_fname ~f:(fun out ->
+            match cli_backend with
+            | `Dot -> Backends.Dot.main out graph
+            | `Verilog -> Backends.Verilog.main out graph)
+     | [] -> parse_error Lexing.dummy_pos "No modules declared")
   with Error { epos; ekind; emsg } ->
-    Printf.eprintf "%s:%d:%d: %s: %s"
-      epos.pos_fname epos.pos_lnum epos.pos_cnum
+    Printf.eprintf "%s:%d:%d: %s: %s\n"
+      epos.pos_fname epos.pos_lnum (epos.pos_cnum - epos.pos_bol)
       (match ekind with
        | `ParseError -> "Parse error"
        | `NameError -> "Name error"
@@ -62,5 +388,40 @@ let run { cli_in_fname; cli_out_fname; cli_backend } : unit =
       emsg;
     exit 1
 
-let main () =
-  Core.Command.run (cli run)
+let backend_of_fname fname =
+  match Core.Filename.split_extension fname with
+  | _, Some "v" -> `Verilog
+  | _, Some "dot" -> `Dot
+  | _, _ -> failwith "Output file must have extension .v or .dot"
+
+let cli =
+  let open Core in
+  Command.basic
+    ~summary:"Compile simultaneous guarded actions to a circuit"
+    Command.Let_syntax.(
+    let%map_open
+        cli_in_fname = anon ("input" %: string)
+    and cli_out_fname = anon ("output" %: string)
+    in fun () ->
+       run { cli_in_fname; cli_out_fname;
+             cli_backend = backend_of_fname cli_out_fname })
+
+let _ =
+  run { cli_in_fname = "collatz.lv"; cli_out_fname = "collatz.v";
+        cli_backend = `Verilog }
+  (* Core.Command.run cli *)
+
+(* let command =
+ *   let open Core in
+ *   Command.basic
+ *     ~summary:"Compile simultaneous guarded actions to a circuit"
+ *     Command.Let_syntax.(
+ *       let%map_open
+ *           cli_in_fname = anon ("input" %: string)
+ *       and cli_out_fname = anon ("output" %: string)
+ *       in
+ *       fun () ->
+ *       Printf.printf "%s %s\n%!" cli_in_fname cli_out_fname)
+ *
+ * let () =
+ *   Core.Command.run command *)
